secure_api/merkle_tree/MerkleTree.New.Low.Hashfunctions.fst
@@ -38,10 +38,15 @@ open MerkleTree.New.Low.Datastructures
 
 #set-options "--z3rlimit 10 --initial_fuel 0 --max_fuel 0 --initial_ifuel 0 --max_ifuel 0"
 
-let init_hash (hsz:hash_size_t) = hash_r_alloc hsz
-let free_hash (hsz:hash_size_t) = hash_r_free #hsz
+let init_hash (hsz:hash_size_t) (r:HST.erid): HST.St (hash #hsz) 
+= rg_alloc (hreg hsz) r
 
-noextract inline_for_extraction unfold
+let free_hash (hsz:hash_size_t) (h:hash #hsz): HST.ST unit
+  (requires (fun h0 -> (Rgl?.r_inv (hreg hsz)) h0 h))
+  (ensures (fun _ _ _ -> True))
+= rg_free (hreg hsz) h
+
+inline_for_extraction
 type hash_fun_t (#hsz:hash_size_t) (#hash_spec:Ghost.erased (MTS.hash_fun_t #(U32.v hsz))) = src1:hash #hsz -> src2:hash #hsz -> dst:hash #hsz -> HST.ST unit
    (requires (fun h0 ->
      Rgl?.r_inv (hreg hsz) h0 src1 /\
